@prefix : <http://purl.org/lis590OD/Fall17/CrimeChargeOnt#> .
@prefix dc: <http://purl.org/dc/elements/1.1/> .
@prefix tl: <http://purl.org/NET/c4dm/timeline.owl#> .
@prefix dbp: <http://dbpedia.org/resource/> .
@prefix geo: <http://www.w3.org/2003/01/geo/wgs84_pos#> .
@prefix org: <http://www.w3.org/ns/org#> .
@prefix owl: <http://www.w3.org/2002/07/owl#> .
@prefix rdf: <http://www.w3.org/1999/02/22-rdf-syntax-ns#> .
@prefix xml: <http://www.w3.org/XML/1998/namespace> .
@prefix xsd: <http://www.w3.org/2001/XMLSchema#> .
@prefix xsp: <http://www.owl-ontologies.com/2005/08/07/xsp.owl#> .
@prefix doco: <https://svn.code.sf.net/p/sempublishing/code/DoCO/doco.owl> .
@prefix foaf: <http://xmlns.com/foaf/0.1/> .
@prefix prov: <http://www.w3.org/ns/prov#> .
@prefix rdfs: <http://www.w3.org/2000/01/rdf-schema#> .
@prefix skos: <http://www.w3.org/2004/02/skos/core#> .
@prefix swrl: <http://www.w3.org/2003/11/swrl#> .
@prefix wped: <http://en.wikipedia.org/wiki/> .
@prefix dolce: <http://ontology.ip.rm.cnr.it/ontologies/DOLCE-Lite#> .
@prefix event: <http://purl.org/NET/c4dm/event.owl#> .
@prefix swrlb: <http://www.w3.org/2003/11/swrlb#> .
@prefix orgrel: <http://purl.org/lis590od/Fall17/OrgRel> .
@prefix dcterms: <http://purl.org/dc/terms/> .
@prefix protege: <http://protege.stanford.edu/plugins/owl/protege#> .
@prefix lkifnorm: <http://www.estrellaproject.org/lkif-core/norm.owl#> .
@prefix lkiflaction: <http://www.estrellaproject.org/lkif-core/action.owl#> .
@prefix lkifexpression: <http://www.estrellaproject.org/lkif-core/expression.owl#> .
@base <http://purl.org/lis590OD/Fall17/CrimeChargeOnt> .

<http://purl.org/lis590OD/Fall17/CrimeChargeOnt> rdf:type owl:Ontology .

#################################################################
#    Object Properties
#################################################################

###  http://purl.org/lis590OD/Fall17/CrimeChargeOnt#Supports
:Supports rdf:type owl:ObjectProperty ;
          owl:inverseOf :isSupportedBy ;
          rdfs:domain lkifexpression:Evidence ;
          rdfs:range :ChargingDocument .


###  http://purl.org/lis590OD/Fall17/CrimeChargeOnt#hasArtifact
:hasArtifact rdf:type owl:ObjectProperty ;
             rdfs:domain lkiflaction:Action ;
             rdfs:range lkifnorm:Legal_Document .


###  http://purl.org/lis590OD/Fall17/CrimeChargeOnt#isSupportedBy
:isSupportedBy rdf:type owl:ObjectProperty ;
               rdfs:domain :ChargingDocument ;
               rdfs:range lkifexpression:Evidence .


###  http://www.essepuntato.it/2008/12/pattern#contains
<http://www.essepuntato.it/2008/12/pattern#contains> rdf:type owl:ObjectProperty ;
                                                     owl:inverseOf <http://www.essepuntato.it/2008/12/pattern#isContainedBy> ;
                                                     rdfs:domain lkifnorm:Code ,
                                                                 lkifnorm:Statute ;
                                                     rdfs:range :CrimeClassification ,
                                                                lkifnorm:Statute .


###  http://www.essepuntato.it/2008/12/pattern#isContainedBy
<http://www.essepuntato.it/2008/12/pattern#isContainedBy> rdf:type owl:ObjectProperty ;
                                                          rdfs:domain lkifnorm:Statute ;
                                                          rdfs:range lkifnorm:Code .


###  http://www.w3.org/2004/02/skos/core#related
skos:related rdf:type owl:ObjectProperty .


###  http://xmlns.com/foaf/0.1/focus
foaf:focus rdf:type owl:ObjectProperty ;
           rdfs:domain foaf:Person ;
           rdfs:range foaf:Person .


###  http://xmlns.com/foaf/0.1/topic
foaf:topic rdf:type owl:ObjectProperty ;
           rdfs:domain lkifnorm:Legal_Document .


#################################################################
#    Classes
#################################################################

###  http://purl.org/lis590OD/Fall17/CrimeChargeOnt#ArrestingCharge
:ArrestingCharge rdf:type owl:Class ;
                 rdfs:subClassOf :Charge ;
                 rdfs:comment "A charge action made at the time of an arrest by the arresting officer. Written down in a police report or other record during booking."@en .


###  http://purl.org/lis590OD/Fall17/CrimeChargeOnt#ArrestingOfficer
:ArrestingOfficer rdf:type owl:Class ;
                  rdfs:subClassOf foaf:Person ;
                  rdfs:comment "An arresting officer is the police department representative who makes an arrest."@en .


###  http://purl.org/lis590OD/Fall17/CrimeChargeOnt#Charge
:Charge rdf:type owl:Class ;
        rdfs:subClassOf lkiflaction:Action ;
        rdfs:comment "An accusation of crime, formulated in a written complaint, information, or indictment, and taking shape in a prosecution."@en .


###  http://purl.org/lis590OD/Fall17/CrimeChargeOnt#ChargingDocument
:ChargingDocument rdf:type owl:Class ;
                  rdfs:subClassOf lkiflaction:Artifact ,
                                  lkifnorm:Legal_Document ;
                  rdfs:comment "From NOLO: A charging document is a pleading that initiates criminal charges against a defendant. It—not arrest—signifies the commencement of a criminal case. Complaints, informations, and indictments are charging documents."@en .


###  http://purl.org/lis590OD/Fall17/CrimeChargeOnt#ConvictingCharge
:ConvictingCharge rdf:type owl:Class ;
                  rdfs:subClassOf :Charge ;
                  rdfs:comment "A charge action made at the time of a conviction by a judge."@en .


###  http://purl.org/lis590OD/Fall17/CrimeChargeOnt#Crime
:Crime rdf:type owl:Class ;
       rdfs:subClassOf skos:Concept ;
       rdfs:comment "A violation of the law."@en .


###  http://purl.org/lis590OD/Fall17/CrimeChargeOnt#CrimeClassification
:CrimeClassification rdf:type owl:Class ;
                     rdfs:comment "Categorization of crimes into misdemeanors, felonies, infractions, and wobblers."@en .


###  http://purl.org/lis590OD/Fall17/CrimeChargeOnt#CrimeCode
:CrimeCode rdf:type owl:Class ;
           rdfs:subClassOf lkifnorm:Legal_Document ;
           rdfs:comment "A crime code is the criminal charge in a written form, typically the section title of a statute"@en .


###  http://purl.org/lis590OD/Fall17/CrimeChargeOnt#CriminalRecord
:CriminalRecord rdf:type owl:Class ;
                rdfs:subClassOf lkifexpression:Evidence ,
                                lkifnorm:Legal_Document ;
                rdfs:comment "A criminal record is documentation of a person's criminal history, including arrests and convictions."@en .


###  http://purl.org/lis590OD/Fall17/CrimeChargeOnt#FormalCharge
:FormalCharge rdf:type owl:Class ;
              rdfs:subClassOf :Charge ;
              rdfs:comment "A charge action made to start the proceedings of a criminal case. Written on a charging document typically by a prosecutor."@en .


###  http://purl.org/lis590OD/Fall17/CrimeChargeOnt#Judge
:Judge rdf:type owl:Class ;
       rdfs:subClassOf foaf:Person ;
       rdfs:comment "From NOLO: An official with the authority and responsibility to preside in a court, try lawsuits, and make legal rulings."@en .


###  http://purl.org/lis590OD/Fall17/CrimeChargeOnt#PoliceReport
:PoliceReport rdf:type owl:Class ;
              rdfs:subClassOf lkiflaction:Artifact ,
                              lkifexpression:Evidence ,
                              lkifnorm:Legal_Document .


###  http://purl.org/lis590OD/Fall17/CrimeChargeOnt#Prosecutor
:Prosecutor rdf:type owl:Class ;
            rdfs:subClassOf foaf:Person ;
            rdfs:comment "From NOLO: A lawyer who works for the local, state, or federal government to bring and litigate criminal cases."@en .


###  http://www.estrellaproject.org/lkif-core/action.owl#Action
lkiflaction:Action rdf:type owl:Class ;
                   rdfs:comment "From LKIF: An action is a change which is brought about by a single agent, playing a role. The agent is the holder of some indended outcome of the action: an action is always intentional. The intention of the agent has usually corresponds with an expectation the intended outcome to be brought about: the agent believes in some expectation. Note that the intention might not correspond with the *actual* outcome of the action."@en .


###  http://www.estrellaproject.org/lkif-core/action.owl#Artifact
lkiflaction:Artifact rdf:type owl:Class ;
                     rdfs:comment "From LKIF: A physical object created by some person to fulfil a particular purpose."@en .


###  http://www.estrellaproject.org/lkif-core/expression.owl#Evidence
lkifexpression:Evidence rdf:type owl:Class ;
                        rdfs:comment "From LKIF: Observation and/or statement, used as a backing for a belief."@en ;
                        rdfs:label "Legal Evidence"@en .


###  http://www.estrellaproject.org/lkif-core/norm.owl#Code
lkifnorm:Code rdf:type owl:Class ;
              rdfs:subClassOf lkifnorm:Legal_Document ;
              rdfs:comment "A code is a collection of statutes and laws organized in some fashion, such as by subject."@en .


###  http://www.estrellaproject.org/lkif-core/norm.owl#Legal_Document
lkifnorm:Legal_Document rdf:type owl:Class ;
                        rdfs:comment "From LKIF: A subclass of a legal source."@en ,
                                     "The legality of a document is most likely related to the fact that a person of the law or legislative body prepared it for some legal purpose."@en .


###  http://www.estrellaproject.org/lkif-core/norm.owl#Statute
lkifnorm:Statute rdf:type owl:Class ;
                 rdfs:subClassOf lkifnorm:Legal_Document ;
                 rdfs:comment "A statute is a formal written enactment of a legislative authority that governs a state, city or country. From LKIF: A statute bears one or more norms, all of which are uttered by some legal person. It cannot bear expressions which are uttered by a different kind of agent."@en .


###  http://www.w3.org/2004/02/skos/core#Concept
skos:Concept rdf:type owl:Class .


###  http://xmlns.com/foaf/0.1/Person
foaf:Person rdf:type owl:Class ;
            rdfs:comment "From FOAF: The Person class represents people. Something is a Person if it is a person. We don't nitpic about whether they're alive, dead, real, or imaginary. The Person class is a sub-class of the Agent class, since all people are considered 'agents' in FOAF."@en .


#################################################################
#    Individuals
#################################################################

###  http://purl.org/lis590OD/Fall17/CrimeChargeOnt#ArrestRecord
:ArrestRecord rdf:type owl:NamedIndividual .


###  http://purl.org/lis590OD/Fall17/CrimeChargeOnt#Complaint
:Complaint rdf:type owl:NamedIndividual ,
                    :ChargingDocument .


###  http://purl.org/lis590OD/Fall17/CrimeChargeOnt#Felony
:Felony rdf:type owl:NamedIndividual ,
                 :CrimeClassification .


###  http://purl.org/lis590OD/Fall17/CrimeChargeOnt#Indictment
:Indictment rdf:type owl:NamedIndividual ,
                     :ChargingDocument .


###  http://purl.org/lis590OD/Fall17/CrimeChargeOnt#Information
:Information rdf:type owl:NamedIndividual ,
                      :ChargingDocument .


###  http://purl.org/lis590OD/Fall17/CrimeChargeOnt#Infraction
:Infraction rdf:type owl:NamedIndividual ,
                     :CrimeClassification .


###  http://purl.org/lis590OD/Fall17/CrimeChargeOnt#Misdemeanor
:Misdemeanor rdf:type owl:NamedIndividual ,
                      :CrimeClassification .


###  http://purl.org/lis590OD/Fall17/CrimeChargeOnt#Ordnance
:Ordnance rdf:type owl:NamedIndividual .


###  http://purl.org/lis590OD/Fall17/CrimeChargeOnt#PoliceReport
:PoliceReport rdf:type owl:NamedIndividual .


###  http://purl.org/lis590OD/Fall17/CrimeChargeOnt#Wobbler
:Wobbler rdf:type owl:NamedIndividual ,
                  :CrimeClassification .


#################################################################
#    Annotations
#################################################################

:PoliceReport rdfs:comment "A police report is a document prepared by a police department representative after an alleged crime has occured. A report can contain information such as the location and date/time of the event, the offender and victim involved, any property impact, and the charge that was allegedly violated."@en .


###  Generated by the OWL API (version 4.2.8.20170104-2310) https://github.com/owlcs/owlapi
